\documentclass{article}
\usepackage{amsmath} % Add missing package
\usepackage{indentfirst} % to indent the first paragraph

\title{2024.3.15 The Second Group Meeting}
\author{Acan Xie}
\date{\today}

\begin{document}

% Title
\maketitle

% Section 1. Introduction
\section{Introduction}

\eqref{eq:1} is ideal gas law equation.

\begin{equation}\label{eq:1}
    PV=NRT
\end{equation}

\eqref{eq:2} is the kinetic energy equation.

\begin{equation}\label{eq:2}
    E = \sum_{i=1}^{N}\frac{|\vec{P_i}|^2}{2m}=H(p,q)
\end{equation}

\eqref{eq:3} is the entropy equation.

\begin{equation}\label{eq:3}
    S=k\ln\omega
\end{equation}

% Section 2. Strling Approximation
\section{Strling Approximation}

According to Mathematical Induction, we can prove \eqref{eq:4}

\begin{equation}\label{eq:4}
    N! = \int_{0}^{\infty} e^{-x}x^Ndx
\end{equation}

Laplace approximation: \eqref{eq:5}

\begin{equation}\label{eq:5}
    \int g(x)dx
\end{equation}

Let $h(x)=\ln g(x)$ then we have

\begin{equation}\label{eq:6}
    \int g(x)dx=\int e^{h(x)}dx
\end{equation}

According to Taylor expansion, we have

\begin{equation}\label{eq:7}
    \int e^{h(x)}dx = \int \exp(h(x_0)+h'(x_0)(x-x_0)+\frac{1}{2}h''(x_0)(x-x_0)^2)dx
\end{equation}

If $h'(x_0)=0$ then we have

\begin{equation}\label{eq:8}
    \begin{aligned}
        \int e^{h(x)} dx &= \int \exp(h(x_0)+\frac{1}{2}h''(x_0)(x-x_0)^2)dx \\ &= e^{h(x_0)} \int \exp (-\frac{1}{2}\frac{(x-x_0)^2}{-h''(x_0)^{-1}})dx
    \end{aligned}
\end{equation}

% Section 3. Energy
\section{Energy}

\end{document}